$Proof Using Taylor Series Expansion
Consider the function 
𝑓
(
𝑡
)
=
(
1
+
𝑡
)
𝑛
f(t)=(1+t) 
n
 .

Step 1: Taylor Series Expansion

The Taylor series expansion of 
𝑓
(
𝑡
)
f(t) around 
𝑡
=
0
t=0 is given by:

𝑓
(
𝑡
)
=
∑
𝑘
=
0
∞
𝑓
(
𝑘
)
(
0
)
𝑘
!
𝑡
𝑘
f(t)= 
k=0
∑
∞
​
  
k!
f 
(k)
 (0)
​
 t 
k
 
Step 2: Compute the Derivatives

First, we need to compute the 
𝑘
k-th derivative of 
𝑓
(
𝑡
)
=
(
1
+
𝑡
)
𝑛
f(t)=(1+t) 
n
 .

Using the chain rule and power rule, the 
𝑘
k-th derivative of 
(
1
+
𝑡
)
𝑛
(1+t) 
n
  is:

𝑓
(
𝑘
)
(
𝑡
)
=
𝑑
𝑘
𝑑
𝑡
𝑘
(
1
+
𝑡
)
𝑛
=
𝑛
!
(
𝑛
−
𝑘
)
!
(
1
+
𝑡
)
𝑛
−
𝑘
f 
(k)
 (t)= 
dt 
k
 
d 
k
 
​
 (1+t) 
n
 = 
(n−k)!
n!
​
 (1+t) 
n−k
 
Evaluating this at 
𝑡
=
0
t=0:

𝑓
(
𝑘
)
(
0
)
=
𝑛
!
(
𝑛
−
𝑘
)
!
f 
(k)
 (0)= 
(n−k)!
n!
​
 
Step 3: Substitute into the Taylor Series

Substitute the 
𝑘
k-th derivative into the Taylor series expansion:

𝑓
(
𝑡
)
=
∑
𝑘
=
0
∞
𝑓
(
𝑘
)
(
0
)
𝑘
!
𝑡
𝑘
=
∑
𝑘
=
0
𝑛
𝑛
!
(
𝑛
−
𝑘
)
!
𝑘
!
𝑡
𝑘
f(t)= 
k=0
∑
∞
​
  
k!
f 
(k)
 (0)
​
 t 
k
 = 
k=0
∑
n
​
  
k!
(n−k)!
n!
​
 
​
 t 
k
 
This simplifies to:

𝑓
(
𝑡
)
=
∑
𝑘
=
0
𝑛
𝑛
!
(
𝑛
−
𝑘
)
!
𝑘
!
𝑡
𝑘
=
∑
𝑘
=
0
𝑛
(
𝑛
𝑘
)
𝑡
𝑘
f(t)= 
k=0
∑
n
​
  
(n−k)!k!
n!
​
 t 
k
 = 
k=0
∑
n
​
 ( 
k
n
​
 )t 
k
 
Since 
𝑓
(
𝑡
)
=
(
1
+
𝑡
)
𝑛
f(t)=(1+t) 
n
 , we have:

(
1
+
𝑡
)
𝑛
=
∑
𝑘
=
0
𝑛
(
𝑛
𝑘
)
𝑡
𝑘
(1+t) 
n
 = 
k=0
∑
n
​
 ( 
k
n
​
 )t 
k
 
Step 4: Apply to 
(
𝑥
+
𝑦
)
𝑛
(x+y) 
n
 

Consider the original binomial expression 
(
𝑥
+
𝑦
)
𝑛
(x+y) 
n
 . To apply the series expansion, we can write:

(
𝑥
+
𝑦
)
𝑛
=
𝑥
𝑛
(
1
+
𝑦
𝑥
)
𝑛
(x+y) 
n
 =x 
n
 (1+ 
x
y
​
 ) 
n
 
Using the series expansion of 
(
1
+
𝑡
)
𝑛
(1+t) 
n
  with 
𝑡
=
𝑦
𝑥
t= 
x
y
​
 :

(
1
+
𝑦
𝑥
)
𝑛
=
∑
𝑘
=
0
𝑛
(
𝑛
𝑘
)
(
𝑦
𝑥
)
𝑘
(1+ 
x
y
​
 ) 
n
 = 
k=0
∑
n
​
 ( 
k
n
​
 )( 
x
y
​
 ) 
k
 
Multiplying both sides by 
𝑥
𝑛
x 
n
 :

𝑥
𝑛
(
1
+
𝑦
𝑥
)
𝑛
=
𝑥
𝑛
∑
𝑘
=
0
𝑛
(
𝑛
𝑘
)
(
𝑦
𝑥
)
𝑘
x 
n
 (1+ 
x
y
​
 ) 
n
 =x 
n
  
k=0
∑
n
​
 ( 
k
n
​
 )( 
x
y
​
 ) 
k
 
(
𝑥
+
𝑦
)
𝑛
=
∑
𝑘
=
0
𝑛
(
𝑛
𝑘
)
𝑥
𝑛
(
𝑦
𝑥
)
𝑘
=
∑
𝑘
=
0
𝑛
(
𝑛
𝑘
)
𝑥
𝑛
−
𝑘
𝑦
𝑘
(x+y) 
n
 = 
k=0
∑
n
​
 ( 
k
n
​
 )x 
n
 ( 
x
y
​
 ) 
k
 = 
k=0
∑
n
​
 ( 
k
n
​
 )x 
n−k
 y 
k
 
Conclusion
This proof correctly uses the Taylor series expansion of 
(
1
+
𝑡
)
𝑛
(1+t) 
n
 , and by substituting 
𝑡
=
𝑦
𝑥
t= 
x
y
​
 , it shows that the expansion of 
(
𝑥
+
𝑦
)
𝑛
(x+y) 
n
  is exactly:

(
𝑥
+
𝑦
)
𝑛
=
∑
𝑘
=
0
𝑛
(
𝑛
𝑘
)
𝑥
𝑛
−
𝑘
𝑦
𝑘
(x+y) 
n
 = 
k=0
∑
n
​
 ( 
k
n
​
 )x 
n−k
 y 
k
 
Thus, the Binomial Theorem is proven using the method of Taylor series expansion. This method is indeed correct and valid.$
